Partial binary search

BinarySearch/Basic.lean
@@ -1,23 +1,86 @@
 import Std.Tactic.BVDecide
 
-def binarySearch {α : Type u} (midpoint : α → α → α) (rangeSize : α → α → Nat)
-    (hr₁ : ∀ a b, 2 ≤ rangeSize a b → rangeSize a (midpoint a b) < rangeSize a b)
-    (hr₂ : ∀ a b, 2 ≤ rangeSize a b → rangeSize (midpoint a b) b < rangeSize a b)
-    (f : α → Bool) (lo hi : α) : α :=
-  match _ : rangeSize lo hi with
-  | 0 => hi
-  | 1 => if f lo then lo else hi
-  | _ + 2 =>
+inductive RangeCheck where
+  | empty
+  | singleton
+  | large
+
+class HasBinarySearch (α : Type u) where
+  checkRange : α → α → RangeCheck
+  rangeSize : α → α → Nat
+  midpoint : α → α → α
+  rangeSize_midpoint_right (lo hi : α) : checkRange lo hi = .large → rangeSize lo (midpoint lo hi) < rangeSize lo hi
+  rangeSize_midpoint_left (lo hi : α) : checkRange lo hi = .large → rangeSize (midpoint lo hi) hi < rangeSize lo hi
+
+open HasBinarySearch
+
+@[specialize]
+def binarySearch {α : Type u} [HasBinarySearch α] (f : α → Bool) (lo hi : α) : α :=
+  match h : checkRange lo hi with
+  | .empty => hi
+  | .singleton => if f lo then lo else hi
+  | .large =>
     let mid := midpoint lo hi
     if f mid then
-      have := hr₁ lo hi
-      binarySearch midpoint rangeSize hr₁ hr₂ f lo mid
+      have := rangeSize_midpoint_right lo hi h
+      binarySearch f lo mid
     else
-      have := hr₂ lo hi
-      binarySearch midpoint rangeSize hr₁ hr₂ f mid hi
+      have := rangeSize_midpoint_left lo hi h
+      binarySearch f mid hi
 termination_by rangeSize lo hi
 
-theorem binarySearch_correct {α : Type u} [LE α] [LT α]
+class MyLinearOrder (α : Type u) extends LE α, LT α where
+  not_le {a b : α} : ¬a ≤ b ↔ b < a
+  le_iff_lt_or_eq {a b : α} : a ≤ b ↔ a < b ∨ a = b
+  lt_trans {a b c : α} : a < b → b < c → a < c
+
+theorem MyLinearOrder.le_or_lt [MyLinearOrder α] {a b : α} : a ≤ b ∨ b < a := by
+  simp [Classical.or_iff_not_imp_left, MyLinearOrder.not_le]
+
+theorem MyLinearOrder.le_refl [MyLinearOrder α] {a : α} : a ≤ a := by
+  simp [le_iff_lt_or_eq]
+
+theorem MyLinearOrder.le_of_lt [MyLinearOrder α] {a b : α} : a < b → a ≤ b := by
+  simp_all [le_iff_lt_or_eq]
+
+theorem MyLinearOrder.le_trans [MyLinearOrder α] {a b c : α} : a ≤ b → b ≤ c → a ≤ c := by
+  rw [le_iff_lt_or_eq, le_iff_lt_or_eq]
+  rintro (hab|rfl) (hbc|rfl)
+  · exact le_of_lt (lt_trans hab hbc)
+  · exact le_of_lt hab
+  · exact le_of_lt hbc
+  · exact le_refl
+
+class HasPartialBinarySearch (α : Type u) extends HasBinarySearch α, MyLinearOrder α where
+  checkRange_eq_empty_iff {lo hi : α} : checkRange lo hi = .empty ↔ hi ≤ lo
+  lt_midpoint {lo hi : α} : checkRange lo hi = .large → lo < midpoint lo hi
+  midpoint_lt {lo hi : α} : checkRange lo hi = .large → midpoint lo hi < hi
+
+theorem HasPartialBinarySearch.le_midpoint {α : Type u} [HasPartialBinarySearch α] {lo hi : α} :
+    checkRange lo hi = .large → lo ≤ midpoint lo hi :=
+  fun h => MyLinearOrder.le_of_lt (lt_midpoint h)
+
+theorem HasPartialBinarySearch.midpoint_le {α : Type u} [HasPartialBinarySearch α] {lo hi : α} :
+    checkRange lo hi = .large → midpoint lo hi ≤ hi :=
+  fun h => MyLinearOrder.le_of_lt (midpoint_lt h)
+
+open HasPartialBinarySearch
+
+def partialBinarySearch {α : Type u} [HasPartialBinarySearch α] (lo hi : α) (f : (a : α) → lo ≤ a → a < hi → Bool) : α :=
+  match h : checkRange lo hi with
+  | .empty => hi
+  | .singleton => if f lo MyLinearOrder.le_refl (by simp [← MyLinearOrder.not_le, ← checkRange_eq_empty_iff, h]) then lo else hi
+  | .large =>
+    let mid := HasBinarySearch.midpoint lo hi
+    if f mid (le_midpoint h) (midpoint_lt h) then
+      have := HasBinarySearch.rangeSize_midpoint_right lo hi h
+      partialBinarySearch lo mid (fun a h₁ h₂ => f a h₁ (MyLinearOrder.lt_trans h₂ (midpoint_lt h)))
+    else
+      have := HasBinarySearch.rangeSize_midpoint_left lo hi h
+      partialBinarySearch mid hi (fun a h₁ h₂ => f a (MyLinearOrder.le_trans (le_midpoint h) h₁) h₂)
+termination_by rangeSize lo hi
+
+/- theorem binarySearch_correct {α : Type u} [LE α] [LT α]
     (lt_of_lt_of_le : ∀ {a b c : α}, a < b → b ≤ c → a < c)
     (lt_of_le_of_lt : ∀ {a b c : α}, a ≤ b → b < c → a < c)
     (lt_irrefl : ∀ (a : α), ¬a < a)
@@ -72,22 +135,55 @@ theorem binarySearch_correct {α : Type u} [LE α] [LT α]
         refine ⟨fun _ => lt_of_lt_of_le hmida ih₂, fun ha hfa => ?_⟩
         exact hmid (hf _ hfa _ (le_of_lt hmida))
       · exact ih₃ _ hmida ha₂
-
+ -/
 section UInt64
 
+@[inline]
+def UInt64.checkRange (lo hi : UInt64) : RangeCheck :=
+  if hi ≤ lo then
+    .empty
+  else if hi - lo = 1 then
+    .singleton
+  else
+    .large
+
+@[inline]
 def UInt64.midpoint (lo hi : UInt64) : UInt64 :=
   lo + (hi - lo) / 2
 
 def UInt64.rangeSize (lo hi : UInt64) : Nat :=
   if lo ≤ hi then (hi - lo).toNat else 0
 
+theorem ite_eq_iff {p : Prop} [Decidable p] {a b c : α} :
+    (if p then a else b) = c ↔ (p ∧ a = c) ∨ (¬ p ∧ b = c) := by
+  split <;> simp_all
+
+theorem helper {lo hi : UInt64} : 2 ≤ (hi - lo).toNat ↔ 2 ≤ hi - lo := by
+  rw [UInt64.le_iff_toNat_le]
+  grind
+
+theorem UInt64.checkRange_eq_empty_iff {lo hi : UInt64} :
+    checkRange lo hi = .empty ↔ hi ≤ lo := by
+  grind [UInt64.checkRange]
+
+theorem UInt64.checkRange_eq_large_iff {lo hi : UInt64} :
+    checkRange lo hi = .large ↔ 2 ≤ rangeSize lo hi := by
+  rw [checkRange, rangeSize]
+  rw [ite_eq_iff]
+  simp only [reduceCtorEq, and_false, UInt64.not_le, ite_eq_right_iff, imp_false, false_or]
+  refine ⟨fun ⟨h₁, h₂⟩ => ?_, ?_⟩
+  · rw [if_pos (by grind), helper]
+    grind
+  · split
+    · rw [helper]
+      grind
+    · simp
+
 theorem UInt64.le_of_rangeSize_pos {lo hi : UInt64} (h : 0 < rangeSize lo hi) : lo ≤ hi := by
   grind [rangeSize]
 
 theorem UInt64.rangeSize_eq_of_pos {lo hi : UInt64} (h : 0 < rangeSize lo hi) : rangeSize lo hi = (hi - lo).toNat := by
   grind [rangeSize]
-
-theorem helper {lo hi : UInt64} (h : lo ≤ hi) (h : 2 ≤ hi - lo) : lo < (lo + (hi - lo) / 2) := by grind
 
 theorem UInt64.rangeSize_midpoint_right (lo hi : UInt64) (h : 2 ≤ rangeSize lo hi) :
     rangeSize lo (midpoint lo hi) < rangeSize lo hi := by
@@ -104,5 +200,53 @@ theorem UInt64.rangeSize_midpoint_left (lo hi : UInt64) (h : 2 ≤ rangeSize lo 
     have : 2 ≤ hi - lo := by simpa [UInt64.le_iff_toNat_le]
     grind
   all_goals grind [rangeSize]
+
+theorem UInt64.lt_midpoint {lo hi : UInt64} (h : 2 ≤ rangeSize lo hi) : lo < UInt64.midpoint lo hi := by
+  simp only [midpoint]
+  have := UInt64.le_of_rangeSize_pos (lo := lo) (hi := hi) (by grind)
+  rw [UInt64.rangeSize_eq_of_pos (by grind), helper] at h
+  grind
+
+theorem UInt64.midpoint_lt {lo hi : UInt64} (h : 2 ≤ rangeSize lo hi) : UInt64.midpoint lo hi < hi := by
+  simp only [midpoint]
+  have := UInt64.le_of_rangeSize_pos (lo := lo) (hi := hi) (by grind)
+  rw [UInt64.rangeSize_eq_of_pos (by grind), helper] at h
+  grind
+
+-- Probably `range_size_midpoint_(right_left)` follow from `lt_midpoint`/`midpoint_lt` in some general setting
+
+instance : HasBinarySearch UInt64 where
+  checkRange := UInt64.checkRange
+  rangeSize := UInt64.rangeSize
+  midpoint := UInt64.midpoint
+  rangeSize_midpoint_right := by
+    simp only [UInt64.checkRange_eq_large_iff]
+    apply UInt64.rangeSize_midpoint_right
+  rangeSize_midpoint_left := by
+    simp only [UInt64.checkRange_eq_large_iff]
+    apply UInt64.rangeSize_midpoint_left
+
+@[inline, specialize]
+def UInt64.binarySearch (f : UInt64 → Bool) (lo hi : UInt64) : UInt64 :=
+  _root_.binarySearch f lo hi
+
+set_option trace.compiler.ir.result true in
+def sqrt (a : UInt64) : UInt64 :=
+  UInt64.binarySearch (fun b => b * b ≥ a) 0 a
+
+instance : MyLinearOrder UInt64 where
+  not_le := UInt64.not_le
+  le_iff_lt_or_eq := UInt64.le_iff_lt_or_eq
+  lt_trans := UInt64.lt_trans
+
+instance : HasPartialBinarySearch UInt64 where
+  checkRange_eq_empty_iff := UInt64.checkRange_eq_empty_iff
+  lt_midpoint := by
+    simp only [checkRange, midpoint, UInt64.checkRange_eq_large_iff]
+    apply UInt64.lt_midpoint
+  midpoint_lt := by
+    simp only [checkRange, midpoint, UInt64.checkRange_eq_large_iff]
+    apply UInt64.midpoint_lt
+
 
 end UInt64
